Split SLC message types into concrete and assertion

tlc/comp/slc.v
@@ -14,80 +14,150 @@ Section slc.
   Variable node : eqType.
   Variable message : eqType.
 
-  (* Requests *)
-
+  (* Concrete requests *)
   Inductive req_sl_ : Type :=
   | Send_sl : node -> message -> req_sl_.
 
   (* Equality *)
+  Section req_sl__eq.
 
-  Definition eq_req_sl_ (r r' : req_sl_) : bool :=
-    match r, r' with
-    | Send_sl n m, Send_sl n' m' => [&& n == n' & m == m']
-    end.
+    Definition eq_req_sl_ (r r' : req_sl_) :=
+      match r, r' with
+      | Send_sl n m, Send_sl n' m' => (n == n') && (m == m')
+      end.
 
-  Lemma eq_req_sl_P : Equality.axiom eq_req_sl_.
-  Proof.
-    case => [ n m ];
-    case => [ n' m' ];
-    rewrite /=; try by constructor.
-    - (* Send_sl *)
-      case Hn: (n == n');
-        [move/eqP: Hn => ?; subst n' | constructor];
-        last by case=> ?; subst n'; rewrite eqxx in Hn.
-      case Hm: (m == m');
-        [move/eqP: Hm => ?; subst m' | constructor];
-        last by case=> ?; subst m'; rewrite eqxx in Hm.
-      by constructor.
-  Qed.
+    Lemma eq_req_sl_P : Equality.axiom eq_req_sl_.
+    Proof.
+      case=> [n m]; case=> [n' m'];
+        rewrite /eq_req_sl_ /=; try by constructor.
+      - (* Send_sl *)
+        case Hn: (n == n');
+          [move/eqP: Hn => ?; subst n' | constructor];
+          last by case=> ?; subst n'; rewrite eqxx in Hn.
+        case Hm: (m == m');
+          [move/eqP: Hm => ?; subst m' | constructor];
+          last by case=> ?; subst m'; rewrite eqxx in Hm.
+        by constructor.
+    Qed.
 
-  Canonical req_sl__eqMixin :=
-    Eval hnf in EqMixin eq_req_sl_P.
-  Canonical req_sl__eqType :=
-    Eval hnf in EqType req_sl_ req_sl__eqMixin.
+    Canonical req_sl__eqMixin :=
+      Eval hnf in EqMixin eq_req_sl_P.
+    Canonical req_sl__eqType :=
+      Eval hnf in EqType req_sl_ req_sl__eqMixin.
 
-  Definition req_sl := [eqType of req_sl_].
+    Definition req_sl := [eqType of req_sl_].
 
-  (* Indications *)
+  End req_sl__eq.
 
+  (* Assertion requests *)
+  Inductive req_sl_A_ : Type :=
+  | Send_sl_A : node_variable -> message_variable -> req_sl_A_.
+
+  (* Equality *)
+  Section req_sl_A__eq.
+
+    Definition eq_req_sl_A_ (r r' : req_sl_A_) :=
+      match r, r' with
+      | Send_sl_A n m, Send_sl_A n' m' => (n == n') && (m == m')
+      end.
+
+    Lemma eq_req_sl_A_P : Equality.axiom eq_req_sl_A_.
+    Proof.
+      case=> [n m]; case=> [n' m'];
+        rewrite /eq_req_sl_A_ /=; try by constructor.
+      - (* Send_sl_A *)
+        case Hn: (n == n');
+          [move/eqP: Hn => ?; subst n' | constructor];
+          last by case=> ?; subst n'; rewrite eqxx in Hn.
+        case Hm: (m == m');
+          [move/eqP: Hm => ?; subst m' | constructor];
+          last by case=> ?; subst m'; rewrite eqxx in Hm.
+        by constructor.
+    Qed.
+
+    Canonical req_sl_A__eqMixin :=
+      Eval hnf in EqMixin eq_req_sl_A_P.
+    Canonical req_sl_A__eqType :=
+      Eval hnf in EqType req_sl_A_ req_sl_A__eqMixin.
+
+    Definition req_sl_A := [eqType of req_sl_A_].
+
+  End req_sl_A__eq.
+
+  (* Concrete indications *)
   Inductive ind_sl_ : Type :=
   | Deliver_sl : node -> message -> ind_sl_.
 
   (* Equality *)
+  Section ind_sl__eq.
 
-  Definition eq_ind_sl_ (i i' : ind_sl_) : bool :=
-    match i, i' with
-    | Deliver_sl n m, Deliver_sl n' m' => [&& n == n' & m == m']
-    end.
+    Definition eq_ind_sl_ (r r' : ind_sl_) :=
+      match r, r' with
+      | Deliver_sl n m, Deliver_sl n' m' => (n == n') && (m == m')
+      end.
 
-  Lemma eq_ind_sl_P : Equality.axiom eq_ind_sl_.
-  Proof.
-    case => [ n m ];
-    case => [ n' m' ];
-    rewrite /=; try by constructor.
-    - (* Deliver_sl *)
-      case Hn: (n == n');
-        [move/eqP: Hn => ?; subst n' | constructor];
-        last by case=> ?; subst n'; rewrite eqxx in Hn.
-      case Hm: (m == m');
-        [move/eqP: Hm => ?; subst m' | constructor];
-        last by case=> ?; subst m'; rewrite eqxx in Hm.
-      by constructor.
-  Qed.
+    Lemma eq_ind_sl_P : Equality.axiom eq_ind_sl_.
+    Proof.
+      case=> [n m]; case=> [n' m'];
+        rewrite /eq_ind_sl_ /=; try by constructor.
+      - (* Deliver_sl *)
+        case Hn: (n == n');
+          [move/eqP: Hn => ?; subst n' | constructor];
+          last by case=> ?; subst n'; rewrite eqxx in Hn.
+        case Hm: (m == m');
+          [move/eqP: Hm => ?; subst m' | constructor];
+          last by case=> ?; subst m'; rewrite eqxx in Hm.
+        by constructor.
+    Qed.
 
-  Canonical ind_sl__eqMixin :=
-    Eval hnf in EqMixin eq_ind_sl_P.
-  Canonical ind_sl__eqType :=
-    Eval hnf in EqType ind_sl_ ind_sl__eqMixin.
+    Canonical ind_sl__eqMixin :=
+      Eval hnf in EqMixin eq_ind_sl_P.
+    Canonical ind_sl__eqType :=
+      Eval hnf in EqType ind_sl_ ind_sl__eqMixin.
 
-  Definition ind_sl := [eqType of ind_sl_].
+    Definition ind_sl := [eqType of ind_sl_].
+
+  End ind_sl__eq.
+
+  (* Assertion indications *)
+  Inductive ind_sl_A_ : Type :=
+  | Deliver_sl_A : node_variable -> message_variable -> ind_sl_A_.
+
+  (* Equality *)
+  Section ind_sl_A__eq.
+
+    Definition eq_ind_sl_A_ (r r' : ind_sl_A_) :=
+      match r, r' with
+      | Deliver_sl_A n m, Deliver_sl_A n' m' => (n == n') && (m == m')
+      end.
+
+    Lemma eq_ind_sl_A_P : Equality.axiom eq_ind_sl_A_.
+    Proof.
+      case=> [n m]; case=> [n' m'];
+        rewrite /eq_ind_sl_A_ /=; try by constructor.
+      - (* Deliver_sl_A *)
+        case Hn: (n == n');
+          [move/eqP: Hn => ?; subst n' | constructor];
+          last by case=> ?; subst n'; rewrite eqxx in Hn.
+        case Hm: (m == m');
+          [move/eqP: Hm => ?; subst m' | constructor];
+          last by case=> ?; subst m'; rewrite eqxx in Hm.
+        by constructor.
+    Qed.
+
+    Canonical ind_sl_A__eqMixin :=
+      Eval hnf in EqMixin eq_ind_sl_A_P.
+    Canonical ind_sl_A__eqType :=
+      Eval hnf in EqType ind_sl_A_ ind_sl_A__eqMixin.
+
+    Definition ind_sl_A := [eqType of ind_sl_A_].
+
+  End ind_sl_A__eq.
 
   (* State *)
-
   Definition slc_state := seq (prod node message).
 
   (* Component *)
-
   Definition slc_subcomps :=
     [:: Subcomp (req_fl node message)
                 (ind_fl node message)].
@@ -112,25 +182,23 @@ Section slc.
       slc_request slc_indication slc_periodic.
 
   (* Specification *)
-
   Section spec.
 
     Import AssertNotations.
 
-    Local Notation Vrn' := (first_var).
-    Local Notation Vrm := (next_var Vrn').
+    Local Notation Vrn' := (first_node_var).
 
     (* Non-compiling
     (* SL_1: Stubborn delivery *)
     Definition SL_1 :=
       ((Pcorrect?(Vrn)) /\ (Pcorrect?(Vrn')) ->
-      (on: Vrn, ev: [], Creq_ev, (Send_sl Vrn' Vrm) =>
-       alwaysf: eventf: on: Vrn', ev: [], Cind_ev, (Deliver_sl Vrn Vrm)))%A.
+      (on: Vrn, ev: [], Creq_ev, (Send_sl_A Vrn' Vrm) =>
+       alwaysf: eventf: on: Vrn', ev: [], Cind_ev, (Deliver_sl_A Vrn Vrm)))%A.
 
     (* SL_2: No-forge *)
     Definition SL_2 :=
-      (on: Vrn, ev: [], Cind_ev, (Deliver_sl Vrn' Vrm) <~
-      on: Vrn', ev: [], Creq_ev, (Send_sl Vrn Vrm))%A.
+      (on: Vrn, ev: [], Cind_ev, (Deliver_sl_A Vrn' Vrm) <~
+      on: Vrn', ev: [], Creq_ev, (Send_sl_A Vrn Vrm))%A.
     *)
 
   End spec.
